starting ze token

tokeneer/token.dfy
@@ -1,12 +1,46 @@
-/*
-A token class, the security level is represented 
-[(low by 1), (medium by 2), (high by 3)]
-
-*/
+datatype clearanceLevel = Low | Medium | High
 
 class Token {
-	var security_level : int;
-	var fingerPrint : int;
+
+	var valifyer : bool
+	var security_level : clearanceLevel;
+	var user_ID	: int
+	
+
+
+constructor (id : int, sec_lvl : clearanceLevel)
+requires id >= 0 	// users always a positive integer
+ensures 		valifyer 
+			&&  user_ID == id 
+			&&  security_level == sec_lvl
+{
+
+valifyer := true;
+security_level := sec_lvl;
+user_ID := id;
+}
+
+
+/*
+requires : that this current token already is valid
+ensures  : that the current token is invalid
+*/
+
+method invalidateToken()
+modifies this`valifyer
+requires valifyer == true
+ensures valifyer == false 
+{
+
+valifyer := false;
+
+}
+
+
+
+
+
+
 
 
 }
